specs

proofs/Challenge1_proof.v
@@ -2,6 +2,8 @@ Set Implicit Arguments.
 (* Load the CFML library. *)
 Require Import CFML.CFLib.
 (* Load the examples CF definitions. *)
+Require Import CFML.Stdlib.Array_proof.
+Require Import CFML.Stdlib.Pervasives_proof.
 Require Import Challenge1_ml.
 
 Require Import TLC.LibInt TLC.LibTactics.
@@ -18,4 +20,54 @@ Ltac auto_tilde ::= rew_list in *; eauto with maths.
 Lemma app_is_app : LibList.app = List.app.
 Admitted.
 Lemma rev_is_rev : rev = List.rev.
+Admitted.
+
+Definition Buf (L1 L2 : list int) gap b :=
+  Hexists l r Ljunk buf,
+    b ~> `{ buf' := buf;
+            l' := (l:int);
+            r' := (r:int) } \*
+    buf ~> Array (rev L1 ++ Ljunk ++ L2) \*
+    \[
+      length L1 = l /\
+      length Ljunk = gap /\
+      r = l + gap
+    ].
+
+Lemma left_spec : forall b L1 L2 gap,
+  app left [b]
+    PRE (b ~> Buf L1 L2 gap)
+    POST (fun (tt:unit) =>
+      match L1 with
+      | nil => b ~> Buf L1 L2 gap
+      | x :: L1' => b ~> Buf L1' (x :: L2) gap
+      end
+    ).
+Admitted.
+
+Lemma right_spec : forall b L1 L2 gap,
+  app right [b]
+    PRE (b ~> Buf L1 L2 gap)
+    POST (fun (tt:unit) =>
+      match L2 with
+      | nil => b ~> Buf L1 L2 gap
+      | x :: L2' => b ~> Buf (x :: L1) L2' gap
+      end
+    ).
+Admitted.
+
+Lemma insert_spec : forall b x L1 L2 (gap:int),
+  app insert [b x]
+    PRE (b ~> Buf L1 L2 gap \* \[gap > 0])
+    POST (fun (tt:unit) => b ~> Buf (x :: L1) L2 (gap - 1)).
+Admitted.
+
+Lemma delete_spec : forall b L1 L2 gap,
+  app delete [b]
+    PRE (b ~> Buf L1 L2 gap)
+    POST (fun (tt:unit) =>
+      match L1 with
+      | nil => b ~> Buf L1 L2 gap
+      | x :: L1' => b ~> Buf L1' L2 (gap + 1)
+      end).
 Admitted.
